murphiGen.py
@@ -1,9 +1,10 @@
 import os
 import argparse
-from abstract import initAbs, doMurphiCheck, test_abs_str
+import csv
+import json
+from abstract import initAbs, test_abs_str
 
-
-arg_parser = argparse.ArgumentParser(description='Learning based CMP')
+arg_parser = argparse.ArgumentParser(description='auto-CMP')
 arg_parser.add_argument('--task', default='mutualEx')
 args = arg_parser.parse_args()
 
@@ -12,21 +13,29 @@ protocol_name = args.task
 #删除旧有的抽象协议
 if os.path.exists('./{0}/ABS{0}.m'.format(protocol_name)):
     os.remove('./{0}/ABS{0}.m'.format(protocol_name))
-#删除旧有的加强记录
-if os.path.exists("{}/{}/abs_process.csv".format(data_dir, protocol_name)):
-    os.remove("{}/{}/abs_process.csv".format(data_dir, protocol_name))
 
-#生成新的抽象协议
+# 生成新的抽象协议
 initAbs("./{0}/{0}.m".format(protocol_name), "./ABS{0}.m".format(protocol_name))
 
-#自动加强
-checked = []
-flag , checked = doMurphiCheck('ABS{}'.format(protocol_name), checked)
+abs_result = dict()    
+csv_f = open('{}/{}/abs_process.csv'.format(data_dir, protocol_name))
+reader = csv.reader(csv_f)
+lemmas = set()
+for line in reader:
+    lemmas |= set(line[1:])
+    abs_result[line[0]] = line[1:]
+invs = []
+for lemma in lemmas:
+    with open('{}/{}/useful_rule/{}.txt'.format(data_dir, protocol_name, lemma), 'r') as f:
+        inv = f.read()
+        invs .append(inv)
+# print(invs)
+with open ("./ABS{0}.m".format(protocol_name), 'a') as  f:
+    for i in invs:
+        f.write(i)
+        f.write('\n')
+csv_f.close()
+for flag, ls in abs_result.items():
+    test_abs_str(flag, name=protocol_name, lemmas=ls)
 
-inv_num = 1
-while flag != None:
-    inv_num = test_abs_str(flag = flag, name = protocol_name,inv_num= inv_num)
-    flag  , checked = doMurphiCheck('ABS{}'.format(protocol_name), checked)
-print("success!")
-
-os.system('mv ./ABS{0}.m ./{0}/'.format(protocol_name))
+os.system('mv {0}/ABS{1}.m {0}/{1}/'.format(data_dir, protocol_name))
