mesi/ABSmesi.m
@@ -17,7 +17,6 @@ var
   state : array [NODE] of LOCATION;
 
 startstate "Init"
-begin
   for i : NODE do
     state[i] := I;
   end;
@@ -135,18 +134,6 @@ begin
   end;
 endrule;
 
-invariant "Lemma_3"
-  forall p : NODE do
-    forall i : NODE do
-      state[i] = MM ->
-        forall j : NODE do
-          j != i ->
-            state[j] != E
-        end
-    end
-  end;
-
-
 invariant "Lemma_4"
   forall p : NODE do
     forall i : NODE do
@@ -159,13 +146,13 @@ invariant "Lemma_4"
   end;
 
 
-invariant "Lemma_5"
+invariant "Lemma_6"
   forall p : NODE do
     forall i : NODE do
-      state[i] = S ->
+      state[i] = MM ->
         forall j : NODE do
           j != i ->
-            state[j] != E
+            state[j] = I
         end
     end
   end;
@@ -183,6 +170,30 @@ invariant "Lemma_0"
   end;
 
 
+invariant "Lemma_3"
+  forall p : NODE do
+    forall i : NODE do
+      state[i] = MM ->
+        forall j : NODE do
+          j != i ->
+            state[j] != E
+        end
+    end
+  end;
+
+
+invariant "Lemma_5"
+  forall p : NODE do
+    forall i : NODE do
+      state[i] = S ->
+        forall j : NODE do
+          j != i ->
+            state[j] != E
+        end
+    end
+  end;
+
+
 invariant "Lemma_9"
   forall p : NODE do
     forall i : NODE do
@@ -190,18 +201,6 @@ invariant "Lemma_9"
         forall j : NODE do
           j != i ->
             state[j] != S
-        end
-    end
-  end;
-
-
-invariant "Lemma_6"
-  forall p : NODE do
-    forall i : NODE do
-      state[i] = MM ->
-        forall j : NODE do
-          j != i ->
-            state[j] = I
         end
     end
   end;
